[crdt] weakening of lub-denot coherence + map_comb (wip)

aneris/examples/crdt/statelib/STS/lst.v
@@ -22,6 +22,18 @@ Section Lst_definition.
   Definition event_set_seqnum_non_O (ls: Lst) :=
     ∀ ev, ev ∈ ls → (O < get_seqnum ev)%nat.
 
+  Record Lst_Validity' (ls: Lst) :=
+    {
+      VLst_same_orig_comp' : event_set_same_orig_comparable ls;
+      VLst_ext_eqid' : events_ext_evid ls;
+      VLst_ext_time' : events_ext_time ls;
+      VLst_orig' : event_set_orig_lt_len ls;
+      VLst_seqnum_non_O' : event_set_seqnum_non_O ls;
+      VLst_orig_max' : event_set_orig_max_len ls;
+      VLst_evid_mon' : event_set_evid_mon ls;
+      VLst_evid_incl_event': event_set_evid_incl_event ls;
+      VLst_evid_incl_time_le': ∀ ev ev', ev ∈ ls → ev' ∈ ls → get_evid ev' ∈ EV_Time ev → ev' ≤_t ev;
+    }.
   Record Lst_Validity (ls: Lst) :=
     {
       VLst_dep_closed : dep_closed ls;
@@ -131,6 +143,114 @@ Section Lst_helper.
     destruct Hmax as (HinM & Ht).
     assert (a = ev ∨ a ≠ ev) as [->| Hneq] by naive_solver; first done.
     epose proof (Ht a _ Hneq); set_solver. Unshelve. by set_solver.
+  Qed.
+
+  Lemma lst_validity'_valid_event_map
+        {Op' : Type} `{!EqDecision Op'} `{!Countable Op'}
+        (s : gset (Event Op))  (f : Op → Op') :
+    Lst_Validity' s  → Lst_Validity' (gset_map (event_map f) s).
+  Proof.
+    destruct 1 as [Hl1 Hl2 Hl3 Hl4 Hl5 Hl6 Hl7 Hl8 Hl9].
+    split.
+    - by apply event_map_is_same_orig_comparable.
+    - intros ev0 ev1 Hev0 Hev1 Heq.
+      pose proof (event_map_elem_of f ev0 s Hev0) as (ev & Hin & Hev).
+      pose proof (event_map_elem_of f ev1 s Hev1) as (ev' & Hin' & Hev').
+      destruct (event_map_inv f ev ev0 Hev) as (HevEq1 & HevEq2 & HevEq3).
+      destruct (event_map_inv f ev' ev1 Hev') as (Hev'Eq1 & Hev'Eq2 & Hev'Eq3).
+      assert (get_evid ev = get_evid ev') as Heqg.
+      { rewrite /get_evid. f_equal; first by naive_solver.
+        rewrite /get_seqnum. naive_solver. }
+      specialize (Hl2 ev ev' Hin Hin' Heqg).
+      by subst.
+    - intros ev0 ev1 Hev0 Hev1 Heq.
+      pose proof (event_map_elem_of f ev0 s Hev0) as (ev & Hin & Hev).
+      pose proof (event_map_elem_of f ev1 s Hev1) as (ev' & Hin' & Hev').
+      destruct (event_map_inv f ev ev0 Hev) as (HevEq1 & HevEq2 & HevEq3).
+      destruct (event_map_inv f ev' ev1 Hev') as (Hev'Eq1 & Hev'Eq2 & Hev'Eq3).
+      assert (EV_Time ev = EV_Time ev') as HeqTime by naive_solver.
+      specialize (Hl3 ev ev' Hin Hin' HeqTime).
+      by subst.
+    - intros ev Hev.
+      pose proof (event_map_elem_of f ev s Hev) as (ev0 & Hin0 & Hev0).
+      destruct (event_map_inv f ev0 ev Hev0) as (Heq1 & Heq2 & Heq3).
+      rewrite -Heq2.
+      by apply Hl4.
+    - intros ev Hev.
+      pose proof (event_map_elem_of f ev s Hev) as (ev0 & Hin0 & Hev0).
+      destruct (event_map_inv f ev0 ev Hev0) as (Heq1 & Heq2 & Heq3).
+      assert (get_seqnum ev = get_seqnum ev0) as -> by naive_solver.
+      by apply Hl5.
+    - intros i Hi.
+      specialize (Hl6 i Hi) as [Hl6|Hl6].
+      -- left. set_solver.
+      -- right.
+         destruct Hl6 as (m & Hm & Hmm).
+         assert ((event_map f m) ∈ gset_map (event_map f) s ∧ EV_Orig ((event_map f m)) = i)
+           as Hfm.
+         {  split; first by set_solver.
+             destruct (event_map_inv f m (event_map f m)) as (Heq1 & Heq2 & Heq3); first done.
+             rewrite -Heq2.
+             apply compute_maximum_correct in Hmm.
+             -- destruct Hmm as (Hmm0 & Hmm1).
+                set_solver.
+             -- intros x y Hx Hy Ht. apply Hl3; set_solver. }
+         assert (∃ m0 : Event Op', compute_maximum (hproj i (gset_map (event_map f) s)) = Some m0)
+           as (m0 & Hm0).
+         { apply (event_set_maximum_exists (gset_map (event_map f) s) i).
+           - exists (event_map f m). apply Hfm.
+           - intros ev0 ev1 Hev0 Hev1 Heq1.
+             pose proof (event_map_elem_of f ev0 s Hev0) as (ev & Hin & Hev).
+             pose proof (event_map_elem_of f ev1 s Hev1) as (ev' & Hin' & Hev').
+             destruct (event_map_inv f ev ev0 Hev) as (HevEq1 & HevEq2 & HevEq3).
+             destruct (event_map_inv f ev' ev1 Hev') as (Hev'Eq1 & Hev'Eq2 & Hev'Eq3).
+             assert (EV_Orig ev = EV_Orig ev') as HeqOrig by naive_solver.
+             specialize (Hl1 ev ev' Hin Hin' HeqOrig).
+             set_solver.
+           -  intros ev0 ev1 Hev0 Hev1 Heq.
+              pose proof (event_map_elem_of f ev0 s Hev0) as (ev & Hin & Hev).
+              pose proof (event_map_elem_of f ev1 s Hev1) as (ev' & Hin' & Hev').
+              destruct (event_map_inv f ev ev0 Hev) as (HevEq1 & HevEq2 & HevEq3).
+              destruct (event_map_inv f ev' ev1 Hev') as (Hev'Eq1 & Hev'Eq2 & Hev'Eq3).
+              assert (EV_Time ev = EV_Time ev') as HeqTime by naive_solver.
+              specialize (Hl3 ev ev' Hin Hin' HeqTime).
+              by subst. }
+         assert ((event_map f) <$> (compute_maximum (hproj i s)) = Some (event_map f m)) as Heq1.
+         by rewrite Hmm.
+         exists m0. split; last done.
+         assert ( ∀ (X : gset (Event Op')) e, compute_maximum X = Some e → e ∈ X) as HeX.
+         { intros X e Hmax.
+           apply elem_of_compute_maximals.
+           rewrite /compute_maximum in Hmax.
+           apply elem_of_elements.
+           destruct (elements (compute_maximals X)) as [|x [|]]; try naive_solver.
+           set_solver.
+         }
+         pose proof (HeX _ m0 Hm0).
+         set_solver.
+    - intros ev0 ev1 Hev0 Hev1 Heq.
+      pose proof (event_map_elem_of f ev0 s Hev0) as (ev & Hin & Hev).
+      pose proof (event_map_elem_of f ev1 s Hev1) as (ev' & Hin' & Hev').
+      destruct (event_map_inv f ev ev0 Hev) as (HevEq1 & HevEq2 & HevEq3).
+      destruct (event_map_inv f ev' ev1 Hev') as (Hev'Eq1 & Hev'Eq2 & Hev'Eq3).
+      assert (EV_Orig ev = EV_Orig ev') as HeqOrig by naive_solver.
+      specialize (Hl7 ev ev' Hin Hin' HeqOrig).
+      by subst.
+    - intros ev Hev.
+      pose proof (event_map_elem_of f ev s Hev) as (ev0 & Hin0 & Hev0).
+      destruct (event_map_inv f ev0 ev Hev0) as (Heq1 & Heq2 & Heq3).
+      specialize (Hl8 ev0 Hin0).
+      assert (get_evid ev0 = get_evid ev) as Heqg.
+      { rewrite /get_evid. f_equal; first by naive_solver.
+        rewrite /get_seqnum. naive_solver. }
+      rewrite Heqg in Hl8.
+      set_solver.
+    - intros ev0 ev1 Hev0 Hev1 Heq.
+      pose proof (event_map_elem_of f ev0 s Hev0) as (ev & Hin & Hev).
+      pose proof (event_map_elem_of f ev1 s Hev1) as (ev' & Hin' & Hev').
+      destruct (event_map_inv f ev ev0 Hev) as (HevEq1 & HevEq2 & HevEq3).
+      destruct (event_map_inv f ev' ev1 Hev') as (Hev'Eq1 & Hev'Eq2 & Hev'Eq3).
+      set_solver.
   Qed.
 
   Lemma lst_validity_valid_event_map
@@ -294,4 +414,12 @@ Section Lst_helper.
       apply (VLst_ext_time _ Hv'' _ _ Hx_in Hy_in).
   Qed.
 
+  Lemma lst_validity_implies_lst_validity' {ls: Lst Op} :
+    Lst_Validity ls → Lst_Validity' ls.
+  Proof.
+    intros[]. repeat split; try assumption.
+    by apply VLst_evid_mon0.
+  Qed.
+
 End Lst_helper.
+
