aneris/examples/crdt/statelib/examples/map_comb/statelib_map_comb_proof.v
@@ -19,6 +19,8 @@ From aneris.examples.crdt.statelib.examples.map_comb
   Require Import statelib_map_comb_code.
 From aneris.examples.crdt.statelib Require Import statelib_code.
 From aneris.aneris_lang.lib Require Import set_proof.
+From aneris.examples.crdt.statelib.proof Require Import events.
+From aneris.examples.crdt.statelib.time Require Import maximality.
 
 Lemma map_dom_None {E E'} `{!EqDecision E, !Countable E} (m: gmap E E') u:
   m !! u = None → u ∉ gset_dom m.
@@ -26,74 +28,28 @@ Proof. by intros?%not_elem_of_dom. Qed.
 Lemma map_dom_Some {E E'} `{!EqDecision E, !Countable E} (m: gmap E E') u v:
   m !! u = Some v → u ∈ gset_dom m.
 Proof. by intros?%elem_of_dom_2. Qed.
+Lemma map_dom_Some_2 {E E'} `{!EqDecision E, !Countable E} (m: gmap E E') u:
+  u ∈ gset_dom m → ∃ v, m !! u = Some v.
+Proof. by intros[]%elem_of_dom; exists x. Qed.
 
-
-Section map_crdt_denot.
-  Context (LogOp : Type) (LogSt : Type).
-  Context `{!Log_Time}.
-  Context `{!EqDecision LogOp} `{!Countable LogOp}.
-  Context `{crdt_denotA : !CrdtDenot LogOp LogSt}.
+Section Bloup.
   Context `{!CRDT_Params}.
+
+  Context (LogOp: Type)
+          (eqdec_logop: EqDecision LogOp) (countable_logop: Countable LogOp).
+  Context (LogSt: Type) (latA: Lattice LogSt).
+  Context (Hcd: @CrdtDenot LogOp LogSt timestamp_time eqdec_logop countable_logop).
+  Context (inj_st: Inject LogSt val).
+
+  Context (p: @StLib_Params LogOp LogSt eqdec_logop countable_logop latA _).
 
   Definition mapSt: Type := gmap string LogSt.
   Definition mapOp: Type := string * LogOp.
 
-  Global Instance map_op_eqdec: EqDecision mapOp.
-  Proof. apply prod_eq_dec. Defined.
-
-  Global Instance map_op_countable: Countable mapOp.
-  Proof. apply prod_countable. Qed.
-
-
-  Definition map_denot_def
-    (s: gset (Event mapOp)) (st: mapSt) : Prop :=
-    gset_dom st = gset_map (λ ev: Event mapOp, ev.(EV_Op).1) s
-    ∧ ∀ (str: string) (v: LogSt), st !! str = Some v →
-      crdt_denot (
-        gset_map
-          (λ e, {|EV_Op := e.(EV_Op).2;
-                  EV_Orig := e.(EV_Orig);
-                  EV_Time := e.(EV_Time) |})
-        (filter (λ ev, ev.(EV_Op).1 = str) s)) v.
-
-  Global Instance map_denot_fun : Rel2__Fun map_denot_def.
-  Proof.
-    constructor. intros s m m' [Hdom Helts][Hdom' Helts'].
-    apply map_eq. intros u.
-    destruct (m !! u)as[v|]eqn:Hms; destruct (m' !! u)as[v'|]eqn:Hm's.
-    - pose proof (Helts u v Hms) as A. pose proof (Helts' u v' Hm's) as B.
-      destruct (crdt_denotA.(crdt_denot_fun))as [Hden].
-      by rewrite Hms Hm's (Hden
-        (gset_map
-        (λ e : Event mapOp,
-           {|
-             EV_Op := (EV_Op e).2; EV_Orig := EV_Orig e; EV_Time := EV_Time e
-           |}) (filter (λ ev : Event (string * LogOp), (EV_Op ev).1 = u) s))
-        v v' A B).
-    - exfalso. rewrite -Hdom in Hdom'.
-      pose proof (map_dom_Some _ _ _ Hms). apply (map_dom_None _ _ Hm's).
-      by rewrite Hdom'.
-    - exfalso. rewrite -Hdom in Hdom'.
-      pose proof (map_dom_Some _ _ _ Hm's). apply (map_dom_None _ _ Hms).
-      by rewrite -Hdom'.
-    - by rewrite Hms Hm's.
-  Qed.
-
-  Global Instance map_crdt_denot: CrdtDenot mapOp mapSt :=
-    {| crdt_denot := map_denot_def |}.
-
-End map_crdt_denot.
-
-Section map_crdt_lattice.
-
-  Context `{latA : !Lattice LogSt}.
-
-  Notation mapSt := (mapSt LogSt).
-
   Definition map_lat_le (st1 st2: mapSt) : Prop :=
     ∀ (s: string) (v: LogSt),
-    st1 !! s = Some v
-    → ∃ (v': LogSt), st2 !! s = Some v' ∧ (latA.(lat_le)) v v'.
+      st1 !! s = Some v
+      → ∃ (v': LogSt), st2 !! s = Some v' ∧ (latA.(lat_le)) v v'.
 
   Definition map_lat_le_po: PartialOrder map_lat_le.
   Proof.
@@ -106,19 +62,18 @@ Section map_crdt_lattice.
       destruct latA as [leA [[reflA trA] AntiSymA] lubA lub_propA].
       by apply (trA v v' v'').
     + intros m m' Hle Hle'.
-      admit.
-      (* apply map_eq. intros s. *)
-      (* destruct (m !! s) as [v|] eqn:E. *)
-      (* - destruct (Hle s v E) as (v' & Heq & Hle_vv'); rewrite Heq. *)
-      (*   destruct (Hle' s v' Heq) as (v'' & Heq' & Hle_v'v). f_equal. *)
-      (*   destruct latA as [leA [[reflA trA] AntiSymA] lubA lub_propA]. *)
-      (*   assert (v'' = v) as ->; first by simplify_eq. *)
-      (*   rewrite Heq'; f_equal. *)
-      (*   by apply (AntiSymA v v'). *)
-      (* - destruct (m' !! s) as [v|] eqn:E'; last by rewrite E E'. *)
-      (*   destruct (Hle' s v E') as (v'' & Ebis & HleA). *)
-      (*   by rewrite Ebis in E. *)
-  Admitted.
+      apply map_eq. intros s.
+      destruct (m !! s) as [v|] eqn:E.
+      - destruct (Hle s v E) as (v' & Heq & Hle_vv'); rewrite Heq.
+        destruct (Hle' s v' Heq) as (v'' & Heq' & Hle_v'v). f_equal.
+        destruct latA as [leA [[reflA trA] AntiSymA] lubA lub_propA].
+        assert (v'' = v) as ->; first by simplify_eq.
+        rewrite Heq'; f_equal.
+        by apply (AntiSymA v v').
+      - destruct (m' !! s) as [v|] eqn:E'; last by rewrite E E'.
+        destruct (Hle' s v E') as (v'' & Ebis & HleA).
+        by rewrite Ebis in E.
+  Qed.
 
   (*Definition map_lat_lub (m m': mapSt) : mapSt :=
     let dom0 := gset_dom m in let dom1 := gset_dom m' in let dom := dom0 ∪ dom1 in
@@ -137,52 +92,206 @@ Section map_crdt_lattice.
           end
         end) (gmap_empty: gmap string LogSt) dom).*)
 
-  Definition map_lat_lub (m m': mapSt): (mapSt) :=
+  Definition map_lat_lub (m m': mapSt): mapSt :=
     map_fold (λ s v' acc,
       match acc !! s with
       | None => map_insert s v' acc
       | Some v => map_insert s (latA.(lat_lub)v v') acc
       end) m m'.
 
+  Lemma TODO1 (m: mapSt):
+    dom m = (gset_dom m).
+  Proof. reflexivity. Qed.
+  Lemma TODO0 i v (m: mapSt):
+    gset_dom (map_insert i v m) = (gset_dom m) ∪ ({[i]}).
+  Proof. do 2rewrite -TODO1.
+    apply set_eq. split; rewrite dom_insert; set_solver. Qed.
+
+  Lemma lat_lub_fold_aux i x (m0: mapSt):
+    ∀ (j1 j2 : string) (z1 z2 : LogSt) (y : mapSt),
+      j1 ≠ j2 → <[i:=x]> m0 !! j1 = Some z1 → <[i:=x]> m0 !! j2 = Some z2 →
+      match match y !! j2 with
+        | Some v0 => map_insert j2 (v0 ⊔_l z2) y
+        | None => map_insert j2 z2 y end !! j1
+      with
+      | Some v0 => map_insert j1 (v0 ⊔_l z1) match y !! j2 with
+        | Some v1 => map_insert j2 (v1 ⊔_l z2) y
+        | None => map_insert j2 z2 y end
+      | None => map_insert j1 z1 match y !! j2 with
+        | Some v0 => map_insert j2 (v0 ⊔_l z2) y
+        | None => map_insert j2 z2 y end end =
+      match match y !! j1 with
+        | Some v0 => map_insert j1 (v0 ⊔_l z1) y
+        | None => map_insert j1 z1 y end !! j2
+      with
+      | Some v0 => map_insert j2 (v0 ⊔_l z2) match y !! j1 with
+        | Some v1 => map_insert j1 (v1 ⊔_l z1) y
+        | None => map_insert j1 z1 y end
+      | None => map_insert j2 z2 match y !! j1 with
+        | Some v0 => map_insert j1 (v0 ⊔_l z1) y
+        | None => map_insert j1 z1 y end end.
+  Proof.
+    intros s1 s2 st1 st2 st Hneq Hs1 Hs2.
+    destruct(st !! s1)as[e1|]eqn:E1; destruct(st !! s2)as[e2|]eqn:E2;
+    destruct(map_insert s2 st2 st !! s1)as[e3|]eqn:E3;
+    try (destruct(map_insert s1 (e1 ⊔_l st1) st !! s2)as[e4|]eqn:E4);
+    try (destruct(map_insert s2 (e2 ⊔_l st2) st !! s1)as[e5|]eqn:E5);
+    try (destruct(map_insert s1 st1 st !! s2)as[e|]eqn:E);
+    apply map_eq; intros s; (destruct (decide (s = s1)); [|destruct(decide(s=s2))]);
+    simplify_eq/=.
+    all: try (rewrite lookup_insert_ne in E3; last done).
+    all: try (rewrite lookup_insert_ne in E4; last done).
+    all: try (rewrite lookup_insert_ne in E5; last done).
+    all: try (rewrite lookup_insert in E3).
+    all: try (rewrite lookup_insert in E4).
+    all: try (rewrite lookup_insert in E5).
+    all: try(rewrite lookup_insert_ne in E; last done).
+    all: try rewrite E5 in E1.
+    all: try rewrite E2 in E4.
+    all: try rewrite E1 in E3.
+    all: try rewrite E in E2.
+    all: simplify_eq/=.
+    all: try ((rewrite lookup_insert lookup_insert_ne; last done);
+      by rewrite lookup_insert).
+    all: by do 4 (rewrite lookup_insert_ne; last done).
+  Qed.
+
+
   Lemma map_lat_lub_dom (m m': mapSt):
     gset_dom (map_lat_lub m m') = (gset_dom m) ∪ (gset_dom m').
   Proof.
-  Admitted.
-  (*   generalize dependent m'. induction m' using map_ind. *)
-  (*   - rewrite/map_lat_lub map_fold_empty. *)
-  (*     replace (gset_dom ∅) with (∅: gset string); *)
-  (*       [ set_solver | by apply set_eq ]. *)
-  (*   - rewrite/map_lat_lub. *)
-  (*     rewrite map_fold_insert; last assumption. *)
-  (* Admitted. *)
+    generalize dependent m'. induction m' using map_ind;
+      first (rewrite /map_lat_lub map_fold_empty;
+      replace (gset_dom ∅) with (∅: gset string);
+        [ set_solver | by apply set_eq ]).
+    rewrite /map_lat_lub map_fold_insert;
+      [ | apply lat_lub_fold_aux | assumption ].
+    apply set_eq. intros s. split.
+    + destruct (m !! i)eqn:E'.
+      * pose proof (iffLR(elem_of_dom (map_lat_lub m m0) i)).
+        rewrite /map_lat_lub in H1.
+        destruct H1 as (elt & Helt).
+        { rewrite TODO1 IHm'. apply elem_of_dom_2 in E'.
+          set_solver. }
+        rewrite Helt TODO0.
+        intros [Hs|Hs%elem_of_singleton]%elem_of_union.
+        --
+          rewrite IHm' in Hs.
+          apply elem_of_union in Hs as [|]; first by apply elem_of_union_l.
+          rewrite TODO0. by apply elem_of_union_r, elem_of_union_l.
+        --
+          rewrite TODO0.
+          by apply elem_of_union_r, elem_of_union_r, elem_of_singleton.
+      * intros Hs.
+        destruct (map_fold (λ s v' acc, match acc !! s with
+              | Some v => map_insert s (v ⊔_l v') acc
+              | None => map_insert s v' acc end) m m0 !! i);
+        rewrite TODO0 IHm' in Hs; rewrite TODO0;
+        apply elem_of_union in Hs as [[Hs|Hs]%elem_of_union|Hs]; set_solver.
+    + destruct (map_fold (λ s v' acc, match acc !! s with
+            | Some v => map_insert s (v ⊔_l v') acc
+            | None => map_insert s v' acc end) m m0 !! i).
+      * intros Hs.
+        rewrite TODO0 in Hs; rewrite TODO0 IHm';
+        apply elem_of_union in Hs as [Hs|[Hs|Hs]%elem_of_union]; set_solver.
+      * intros Hs. rewrite TODO0 in Hs. rewrite TODO0 IHm'. set_solver.
+  Qed.
 
-  Lemma map_lub_elt_Some_Some (m m': gmap string LogSt) (s: string)
-    (v v': LogSt):
-    m !! s = Some v → m' !! s = Some v' →
-    (map_lat_lub m m') !! s = Some (latA.(lat_lub) v v').
+  Lemma map_lub_elts (m m': gmap string LogSt) (s: string):
+    (∀ v v',
+      m !! s = Some v → m' !! s = Some v'
+        → (map_lat_lub m m') !! s = Some (latA.(lat_lub) v v'))
+    ∧ (∀ (v: LogSt),
+        m !! s = Some v → m' !! s = None →
+        (map_lat_lub m m') !! s = Some v)
+    ∧ (∀ (v: LogSt),
+        m !! s = None → m' !! s = Some v →
+        (map_lat_lub m m') !! s = Some v)
+    ∧ (m !! s = None → m' !! s = None → (map_lat_lub m m') !! s = None).
   Proof.
-    generalize dependent m';
     generalize dependent s;
-    generalize dependent v;
-    generalize dependent v';
-    generalize dependent m.
-    induction m as [|s' v'' m Hm's' IH] using map_ind; first inversion 1.
-    intros v' v s m' Hms Hm's.
-  Admitted.
+    generalize dependent m'; induction m' using map_ind;
+      first (intros s; split; first inversion 2;
+      intros; by rewrite/map_lat_lub map_fold_empty).
+    rewrite /map_lat_lub map_fold_insert;
+      [ | apply lat_lub_fold_aux | assumption ].
+    set IHSS := λ e, proj1 (IHm' e).
+    set IHSN := λ e, proj1(proj2 (IHm' e)).
+    set IHNS := λ e, proj1(proj2(proj2 (IHm' e))).
+    set IHNN := λ e, proj2(proj2(proj2 (IHm' e))).
+    intros s; repeat split.
+    * intros v v' Hms Hm0's.
+      destruct(decide(i = s))as[-> | ].
+      - rewrite (IHSN s v); try done.
+        rewrite lookup_insert. by rewrite lookup_insert in Hm0's; simplify_eq/=.
+      - destruct(m !! i)as[l|]eqn:E.
+        + rewrite (IHSN i l E H0) lookup_insert_ne; last done.
+          rewrite lookup_insert_ne in Hm0's; last done.
+          by apply (IHSS s).
+        + rewrite lookup_insert_ne in Hm0's; last done.
+          pose proof (IHm' s)as [IHm'1 IHm'2].
+          rewrite (IHNN _ E H0)
+            lookup_insert_ne; last done.
+          by apply IHSS.
+    * intros v Hms Hm0's.
+      destruct(decide(i = s))as[-> | ].
+      - rewrite (IHSN s v); try done.
+        rewrite lookup_insert. by rewrite lookup_insert in Hm0's; simplify_eq/=.
+      - destruct(m !! i)as[l|]eqn:E.
+        + rewrite (IHSN i l E H0) lookup_insert_ne; last done.
+          rewrite lookup_insert_ne in Hm0's; last done.
+          by apply IHSN.
+        + rewrite lookup_insert_ne in Hm0's; last done.
+          rewrite (IHNN _ E H0) lookup_insert_ne; last done.
+          by apply IHSN.
+    * intros v Hms Hm0s.
+      destruct(decide(i = s))as[-> | ].
+      - rewrite (IHNN _ Hms H0)lookup_insert.
+        by rewrite lookup_insert in Hm0s.
+      - destruct(m !! i)as[l|]eqn:E.
+        + rewrite lookup_insert_ne in Hm0s; last done.
+          rewrite (IHSN i _ E H0) lookup_insert_ne; last done.
+          by apply IHNS.
+        + rewrite lookup_insert_ne in Hm0s; last done.
+          rewrite (IHNN i E H0) lookup_insert_ne; last done.
+          by apply IHNS.
+    * intros Hms Hm0's.
+      destruct(decide(i = s))as[-> | ].
+      - by rewrite lookup_insert in Hm0's; simplify_eq/=.
+      - destruct(m !! i)as[l|]eqn:E.
+        + rewrite (IHSN i _ E H0) lookup_insert_ne; last done.
+          apply IHNN; try done.
+          by rewrite lookup_insert_ne in Hm0's.
+        + rewrite lookup_insert_ne in Hm0's; last done.
+          rewrite (IHNN _ E H0) lookup_insert_ne; last done.
+          by apply IHNN.
+  Qed.
+
+  Lemma map_lub_elt_None_None (m m': gmap string LogSt) (s: string):
+    m !! s = None → m' !! s = None → (map_lat_lub m m') !! s = None.
+  Proof.
+    destruct (map_lub_elts m m' s) as (_&_&_&HNN). intros. by apply HNN. Qed.
+
+  Lemma map_lub_elt_None_Some (m m': gmap string LogSt) (s: string)
+    (v: LogSt):
+    m' !! s = Some v → m !! s = None →
+    (map_lat_lub m m') !! s = Some v.
+  Proof.
+    destruct (map_lub_elts m m' s) as (_&_&HNS&_). intros. by apply HNS. Qed.
 
   Lemma map_lub_elt_Some_None (m m': gmap string LogSt) (s: string)
     (v: LogSt):
     m !! s = Some v → m' !! s = None →
     (map_lat_lub m m') !! s = Some v.
-    Admitted.
-  Lemma map_lub_elt_None_Some (m m': gmap string LogSt) (s: string)
-    (v: LogSt):
-    m' !! s = Some v → m !! s = None →
-    (map_lat_lub m m') !! s = Some v.
-    Admitted.
-  Lemma map_lub_elt_None_None (m m': gmap string LogSt) (s: string):
-    m !! s = None → m' !! s = None → (map_lat_lub m m') !! s = None.
-    Admitted.
+  Proof.
+    destruct (map_lub_elts m m' s) as (_&HSN&_&_). intros. by apply HSN. Qed.
+
+  Lemma map_lub_elt_Some_Some {m m': gmap string LogSt}{s: string}
+    {v v': LogSt}:
+    m !! s = Some v → m' !! s = Some v' →
+    (map_lat_lub m m') !! s = Some (v ⊔_l v').
+  Proof.
+    destruct (map_lub_elts m m' s) as (HSS&_&_&_). intros. by apply HSS. Qed.
 
   Global Instance map_lattice: Lattice (gmap string LogSt).
   Proof.
@@ -195,14 +304,14 @@ Section map_crdt_lattice.
     - intros s v Hms.
       destruct(m' !! s) as [v' | ] eqn:Hm's.
       + exists (latA.(lat_lub) v v').
-        rewrite (map_lub_elt_Some_Some m m' s v v' Hms Hm's).
+        rewrite (map_lub_elt_Some_Some Hms Hm's).
         split; first trivial.
         by apply lat_lub_le_l.
       + exists v. by rewrite (map_lub_elt_Some_None m m' s v Hms Hm's).
     - intros s v' Hm's.
       destruct (m !! s) as [ v | ] eqn:Hms.
       + exists (latA.(lat_lub) v v').
-        rewrite (map_lub_elt_Some_Some _ _ _ _ _ Hms Hm's).
+        rewrite (map_lub_elt_Some_Some Hms Hm's).
         split; first trivial. by apply lat_lub_le_r.
       + exists v'. by rewrite (map_lub_elt_None_Some _ _ _ _ Hm's Hms).
     - intros m'' Hle Hle' s vlub Hlubs.
@@ -211,7 +320,7 @@ Section map_crdt_lattice.
         pose proof (Hle' s v' Hm's) as (v''_bis & Hv''_bis & Hle''_bis).
         assert(v''_bis = v'') as ->. { by simplify_eq. }
         exists v''. split; first trivial.
-        rewrite (map_lub_elt_Some_Some _ _ _ _ _ Hms Hm's) in Hlubs.
+        rewrite (map_lub_elt_Some_Some Hms Hm's) in Hlubs.
         simplify_eq. by apply lat_lub_le.
       + pose proof (Hle s v Hms) as (v'' & Hv'' & Hle'').
         exists v''. split; first trivial.
@@ -224,77 +333,43 @@ Section map_crdt_lattice.
       + by rewrite (map_lub_elt_None_None _ _ _ Hms Hm's) in Hlubs.
   Defined.
 
-End map_crdt_lattice.
+  Global Instance map_op_eqdec: EqDecision mapOp.
+  Proof. apply prod_eq_dec. Defined.
 
-Section map_crdt_coh_params.
+  Global Instance map_op_countable: Countable mapOp.
+  Proof. apply prod_countable. Qed.
 
-  Context (LogOp : Type) (LogSt : Type).
-  Context `{!EqDecision LogOp} `{!Countable LogOp}.
-  Context `{!Inject LogOp val} `{!Inject LogSt val}.
-  Context `{!anerisG M Σ}.
-  Context `{!CRDT_Params}.
-  Context `{p : !@StLib_Coh_Params LogOp LogSt}.
-  Notation mapOp := (mapOp LogOp).
-  Notation mapSt := (mapSt LogSt).
+  Definition map_denot_def
+    (s: gset (Event mapOp)) (st: mapSt) : Prop :=
+    gset_dom st = gset_map (λ ev: Event mapOp, ev.(EV_Op).1) s
+    ∧ (∀ (str: string) (v: LogSt), st !! str = Some v →
+      @crdt_denot LogOp LogSt timestamp_time eqdec_logop countable_logop
+      p.(StLib_Denot)
+      (gset_map
+          (λ e, {|EV_Op := e.(EV_Op).2;
+                  EV_Orig := e.(EV_Orig);
+                  EV_Time := e.(EV_Time) |})
+        (filter (λ ev, ev.(EV_Op).1 = str) s)) v).
 
-  (** serialization *)
-  Definition map_ser : serialization :=
-    list_serialization
-      (prod_serialization
-        string_serialization p.(StLib_StSerialization)).
-
-  Definition map_op_coh (op: mapOp) (v: val): Prop :=
-    ∃(s: string)(lop: LogOp)(vs vop: val),
-      op.1 = s ∧ op.2 = lop
-      ∧ v = (vs, vop)%V
-      ∧ p.(StLib_Op_Coh) lop vop
-      ∧ vs = #s.
-
-  Definition map_st_coh (st: mapSt) (v: val): Prop := is_map v st.
-
-  Lemma map_coh_ser:
-    ∀ (st : mapSt) (v : val), map_st_coh st v → Serializable map_ser v.
-    Admitted.
-
-  Global Instance map_crdt_coh_params : @StLib_Coh_Params mapOp mapSt.
+  Global Instance map_denot_fun : Rel2__Fun map_denot_def.
   Proof.
-    refine {|
-      StLib_StSerialization := map_ser;
-      StLib_Op_Coh := map_op_coh;
-      StLib_St_Coh := map_st_coh;
-       |}.
-    - intros [ol or][ol' or'] v
-        (s & lop & vs & vop & Hseq & Hlopeq & Hveq & Hlopcoh & Hvsq)
-        (s'& lop'& vs'& vop'& Hseq'& Hlopeq'& Hveq'& Hlopcoh'& Hvsq').
-      f_equal; first by simplify_eq/=.
-      simplify_eq/=. by apply (p.(StLib_Op_Coh_Inj)lop lop' vop').
-    - intros st st' v (l&->&Hl&H'l)(l'&->&Hl'&H'l').
-      assert(l=l') as ->; last reflexivity.
-      rewrite Hl in Hl'. by apply inject_inj.
-    - exact map_coh_ser.
-  Defined.
+    constructor. intros s m m' (Hdom&Helts)(Hdom'&Helts').
+    apply map_eq. intros u.
+    destruct (m !! u)as[v|]eqn:Hms; destruct (m' !! u)as[v'|]eqn:Hm's.
+    - pose proof (Helts u v Hms) as A. pose proof (Helts' u v' Hm's) as B.
+      rewrite Hms Hm's. f_equal.
+      exact (p.(StLib_Denot).(crdt_denot_fun).(rel2_fun)A B).
+    - exfalso. rewrite -Hdom in Hdom'.
+      pose proof (map_dom_Some _ _ _ Hms). apply (map_dom_None _ _ Hm's).
+      by rewrite Hdom'.
+    - exfalso. rewrite -Hdom in Hdom'.
+      pose proof (map_dom_Some _ _ _ Hm's). apply (map_dom_None _ _ Hms).
+      by rewrite -Hdom'.
+    - by rewrite Hms Hm's.
+  Qed.
 
-End map_crdt_coh_params.
-
-Section map_crdt_model.
-
-  (* Context `{latA: Lattice LogSt, !EqDecision LogOp, !Countable LogOp, *)
-  (*           !@CrdtDenot LogOp LogSt timestamp_time _ _, !CRDT_Params, *)
-  (*           inj_st: Inject LogSt val}. *)
-  (* Context {p: StLib_Params LogOp LogSt}. *)
-
-  Context (LogOp : Type) (LogSt : Type).
-  Context `{!EqDecision LogOp}.
-  Context `{!Countable LogOp}.
-  Context `{!Inject LogOp val}.
-  Context `{!Inject LogSt val}.
-  Context `{!anerisG M Σ}.
-  Context `{!CRDT_Params}.
-  Context `{latA : !Lattice LogSt}.
-  Context `{crdt_denotA : !CrdtDenot LogOp LogSt}.
-  Context `{PA : !StateCrdtModel LogOp LogSt}.
-  Notation mapOp := (mapOp LogOp).
-  Notation mapSt := (mapSt LogSt).
+  Global Instance map_denot: CrdtDenot mapOp mapSt :=
+    {| crdt_denot := map_denot_def |}.
 
   Definition map_event (e: Event mapOp) : Event LogOp :=
     {|EV_Orig := EV_Orig e;
@@ -302,7 +377,7 @@ Section map_crdt_model.
       EV_Time := EV_Time e;
     |}.
 
-  (* Context `{PA : !StLib_Params LogOp LogSt}. *)
+  Context `{PA : !StLib_Params LogOp LogSt}.
 
   Definition map_mutator (m: mapSt) (e: Event mapOp) (m': mapSt) : Prop :=
     let key: string := e.(EV_Op).1 in
@@ -311,75 +386,127 @@ Section map_crdt_model.
     ∧ (∀ k v, k ≠ key → m !! k = Some v → m' !! k = Some v)
     ∧ (∀ (v: LogSt),
         m !! key = Some v →
-        ∃ v', PA.(st_crdtM_mut) v (map_event e) v'
+        ∃ v', PA.(StLib_Model).(st_crdtM_mut) v (map_event e) v'
           ∧ m' !! key = Some v')
     ∧ (m !! key = None →  ∃ (v': LogSt),
-        PA.(st_crdtM_mut)
-          PA.(st_crdtM_init_st) (map_event e) v' ∧
+        PA.(StLib_Model).(st_crdtM_mut)
+          PA.(StLib_Model).(st_crdtM_init_st) (map_event e) v' ∧
         m' !! key = Some v').
+
+  Definition map_event_map :=
+    λ e : Event (string * LogOp),
+       {|
+         EV_Op := (EV_Op e).2;
+         EV_Orig := EV_Orig e;
+         EV_Time := EV_Time e
+       |}.
+
+  Lemma lst_val_map s lst:
+    Lst_Validity' lst →
+    Lst_Validity'
+      (gset_map map_event_map
+        (filter (λ ev : Event (string * LogOp), (EV_Op ev).1 = s) lst)).
+  Proof.
+    destruct 1.
+    apply (lst_validity'_valid_event_map). split;
+    try intros ??[_?]%elem_of_filter[_?]%elem_of_filter;
+    try intros?[_?]%elem_of_filter;
+    [ by apply VLst_same_orig_comp'
+    | by apply VLst_ext_eqid'
+    | by apply VLst_ext_time'
+    | by apply VLst_orig'
+    | by apply VLst_seqnum_non_O'
+    | | by apply VLst_evid_mon'
+    | by apply VLst_evid_incl_event'
+    | by apply VLst_evid_incl_time_le' ].
+    - intros??.
+      destruct
+        (set_choose_or_empty(hproj i(filter (λ ev, (EV_Op ev).1 = s) lst)));
+        [right | by left].
+      destruct (compute_maximum_non_empty
+        (hproj i (filter (λ ev, (EV_Op ev).1 = s) lst))).
+      + intros??[?[_?]%elem_of_filter]%elem_of_filter
+          [?[_?]%elem_of_filter]%elem_of_filter.
+        apply VLst_same_orig_comp'; [done|done|lia].
+      + intros??[?[_?]%elem_of_filter]%elem_of_filter
+          [?[_?]%elem_of_filter]%elem_of_filter.
+        by apply VLst_ext_time'.
+      + destruct H2 as[x Hx]; first set_solver.
+        exists x. split; last done.
+        apply compute_maximum_correct in Hx as [??]; last first.
+        intros??[?[??]%elem_of_filter]%elem_of_filter
+          [?[??]%elem_of_filter]%elem_of_filter.
+        by apply VLst_ext_time'.
+        apply elem_of_filter; set_solver.
+  Qed.
 
   Lemma map_mut_lub_coh:
     ∀ (s1 s2 : event_set mapOp) (st1 st2 st3 : mapSt),
       ⟦ s1 ⟧ ⇝ st1
       → ⟦ s2 ⟧ ⇝ st2
-        → Lst_Validity s1
-          → Lst_Validity s2
-            → Lst_Validity (s1 ∪ s2) → st1 ⊔_l st2 = st3 → ⟦ s1 ∪ s2 ⟧ ⇝ st3.
+      → Lst_Validity' s1
+      → Lst_Validity' s2 → Lst_Validity' (s1 ∪ s2)
+      → (∀ i : nat, fil s1 i ⊆ fil s2 i ∨ fil s2 i ⊆ fil s1 i)
+      → st1 ⊔_l st2 = st3 → ⟦ s1 ∪ s2 ⟧ ⇝ st3.
   Proof.
-    intros s1 s2 st1 st2?[Hdom1 Hden1][Hdom2 Hden2]Hv1 Hv2 Hv3<-.
-    split; first by rewrite map_lat_lub_dom Hdom1 Hdom2 gset_map_union.
+    intros s1 s2 st1 st2 st3[Hdom Hden][Hdom' Hden']Hv1 Hv2 Hv3 Hproj <-.
+    split; first by rewrite map_lat_lub_dom Hdom Hdom' gset_map_union.
     intros s v Hs.
+    set mapped_s1 := gset_map
+      (λ e : Event (string * LogOp),
+      {| EV_Op := (EV_Op e).2; EV_Orig := EV_Orig e; EV_Time := EV_Time e |})
+      (filter (λ ev : Event (string * LogOp), (EV_Op ev).1 = s) s1).
+    set mapped_s2 := gset_map
+      (λ e : Event (string * LogOp),
+      {| EV_Op := (EV_Op e).2; EV_Orig := EV_Orig e; EV_Time := EV_Time e |})
+      (filter (λ ev : Event (string * LogOp), (EV_Op ev).1 = s) s2).
+    set mapped_s12 := gset_map
+      (λ e : Event (string * LogOp),
+      {| EV_Op := (EV_Op e).2; EV_Orig := EV_Orig e; EV_Time := EV_Time e |})
+      (filter (λ ev : Event (string * LogOp), (EV_Op ev).1 = s) (s1 ∪ s2)).
     destruct (st1 !! s) as [l |] eqn:E;
-    destruct (st2 !! s) as [l' |] eqn:E'.
-    (* last (exfalso; pose proof (map_lub_elt_None_None st1 st2 s E E');
-      by rewrite H1 in Hs). *)
-    - pose proof (map_lub_elt_Some_Some st1 st2 s l l' E E').
-      replace (gset_map
-        (λ e : Event (string * LogOp),
-           {| EV_Op := (EV_Op e).2; EV_Orig := EV_Orig e; EV_Time := EV_Time e |})
-        (filter (λ ev : Event (string * LogOp), (EV_Op ev).1 = s) (s1 ∪ s2)))
-        with (
-          (gset_map
-                (λ e : Event (string * LogOp),
-                   {|
-                     EV_Op := (EV_Op e).2;
-                     EV_Orig := EV_Orig e;
-                     EV_Time := EV_Time e
-                   |})
-                (filter (λ ev : Event (string * LogOp), (EV_Op ev).1 = s)
-                   s1))
-          ∪ (gset_map
-                (λ e : Event (string * LogOp),
-                   {|
-                     EV_Op := (EV_Op e).2;
-                     EV_Orig := EV_Orig e;
-                     EV_Time := EV_Time e
-                   |})
-                (filter (λ ev : Event (string * LogOp), (EV_Op ev).1 = s)
-                   s2))); last set_solver.
-      specialize Hden1 with s l.
-      (*pose proof (p.(StLib_Model).(st_crdtM_lub_coh)
-        (gset_map
-          (λ e : Event (string * LogOp),
-             {| EV_Op := (EV_Op e).2; EV_Orig := EV_Orig e; EV_Time := EV_Time e |})
-          (filter (λ ev : Event (string * LogOp), (EV_Op ev).1 = s) s1))
-        (gset_map
-          (λ e : Event (string * LogOp),
-             {| EV_Op := (EV_Op e).2; EV_Orig := EV_Orig e; EV_Time := EV_Time e |})
-          (filter (λ ev : Event (string * LogOp), (EV_Op ev).1 = s) s2))
-        l l' (l ⊔_l l') (Hden1 E)).*) admit.
-    - admit.
-    - admit.
-    - admit.
-  Admitted.
+    destruct (st2 !! s) as [l' |] eqn:E';
+    last (exfalso; pose proof (map_lub_elt_None_None st1 st2 s E E');
+      by rewrite H0 in Hs).
+    - pose proof (map_lub_elt_Some_Some E E').
+      replace mapped_s12 with (mapped_s1 ∪ mapped_s2); last set_solver.
+      pose proof (Hden s l E) as H1; pose proof (Hden' s l' E') as H2.
+      rewrite-/mapped_s1 in H1; rewrite-/mapped_s2 in H2.
+      apply (p.(StLib_Model).(st_crdtM_lub_coh)_ _ _ _ _ H1 H2).
+      + by apply lst_val_map.
+      + by apply lst_val_map.
+      + assert((mapped_s1 ∪ mapped_s2) = mapped_s12) as Hseq; first set_solver.
+        rewrite Hseq. by apply lst_val_map.
+      + rewrite Hs in H0.
+        intros i. destruct (Hproj i); [left | right]; set_solver.
+      + rewrite(map_lub_elt_Some_Some E E') in Hs. by simplify_eq/=.
+    - pose proof (map_lub_elt_Some_None st1 st2 s l E E')as H0.
+      replace mapped_s12 with (mapped_s1 ∪ mapped_s2); last set_solver.
+      pose proof (Hden s l E) as H1.
+      rewrite-/mapped_s1 in H1.
+      assert(mapped_s2 = ∅) as ->.
+      { apply map_dom_None in E'. set_solver. }
+      rewrite Hs in H0. simplify_eq/=.
+      replace (mapped_s1 ∪ ∅) with mapped_s1; [assumption | set_solver].
+    - pose proof (map_lub_elt_None_Some st1 st2 s l' E' E)as H0.
+      replace mapped_s12 with (mapped_s1 ∪ mapped_s2); last set_solver.
+      pose proof (Hden' s l' E') as H2.
+      rewrite-/mapped_s2 in H2.
+      assert(mapped_s1 = ∅) as ->.
+      { apply map_dom_None in E. set_solver. }
+      rewrite Hs in H0. simplify_eq/=.
+      replace (∅ ∪ mapped_s2) with mapped_s2; [assumption | set_solver].
+  Qed.
 
   Lemma map_mut_coh:
     ∀ (s : event_set mapOp) (st st' : mapSt) (ev : Event mapOp),
       ⟦ s ⟧ ⇝ st
       → Lst_Validity s
-        → ev ∉ s
-          → is_maximum ev (s ∪ {[ev]})
-            → map_mutator st ev st' → ⟦ s ∪ {[ev]} ⟧ ⇝ st'. Admitted.
+      → ev ∉ s
+      → is_maximum ev (s ∪ {[ev]})
+      → map_mutator st ev st' → ⟦ s ∪ {[ev]} ⟧ ⇝ st'.
+  Proof.
+  Admitted.
 
   Lemma map_mut_mon (m : mapSt) (e : Event mapOp) (m' : mapSt) :
     map_mutator m e m' → m ≤_l m'.
@@ -388,11 +515,12 @@ Section map_crdt_model.
     destruct(decide(s = (EV_Op e).1)) as[-> | ].
     + destruct (Hnew_v _ Hmsv)as(v'&Hmut&Hm'sv').
       exists v'. split; first assumption.
-      by apply st_crdtM_mut_mon with (map_event e).
+      apply st_crdtM_mut_mon with (map_event e).
+      apply Hmut.
     + exists v. split; last done. exact (Hold_v s v n Hmsv).
   Qed.
 
-  Global Instance map_crdt_model : StateCrdtModel mapOp mapSt.
+  Global Instance map_model : StateCrdtModel mapOp mapSt.
   Proof.
     refine {| st_crdtM_lub_coh := map_mut_lub_coh;
               st_crdtM_mut_mon := map_mut_mon;
@@ -402,50 +530,66 @@ Section map_crdt_model.
     split; [ by apply set_eq | inversion 1 ].
   Defined.
 
-End map_crdt_model.
 
-Section map_crdt_params.
 
-  Context (LogOp : Type) (LogSt : Type).
-  Context `{!EqDecision LogOp} `{!Countable LogOp}.
-  Context `{!anerisG M Σ}.
-  Context `{!CRDT_Params}.
-  Context `{!Lattice LogSt}.
-  Context `{!Inject LogOp val}.
-  Context `{!Inject LogSt val}.
-  Context `{!StLib_Params LogOp LogSt}.
+  (** serialization *)
+  Definition map_ser : serialization :=
+    list_serialization
+      (prod_serialization
+        string_serialization p.(StLib_CohParams).(StLib_StSerialization)).
 
-  Notation mapOp := (mapOp LogOp).
-  Notation mapSt := (mapSt LogSt).
+  Definition map_op_coh (op: mapOp) (v: val): Prop :=
+    ∃(s: string)(lop: LogOp)(vs vop: val),
+      op.1 = s ∧ op.2 = lop
+      ∧ v = (vs, vop)%V
+      ∧ p.(StLib_CohParams).(StLib_Op_Coh) lop vop
+      ∧ vs = #s.
 
-  Global Instance map_crdt_params :
-   StLib_Params mapOp mapSt :=
-    {
-      StLib_Denot           := map_crdt_denot LogOp LogSt;
-      StLib_Model           := map_crdt_model LogOp LogSt;
-      StLib_CohParams       := map_crdt_coh_params LogOp LogSt;
-    }.
+  Definition map_st_coh (st: mapSt) (v: val): Prop := is_map v st.
 
-End map_crdt_params.
+  Lemma map_coh_ser:
+    ∀ (st : mapSt) (v : val), map_st_coh st v → Serializable map_ser v.
+    Admitted.
+
+  Global Instance map_coh_params : @StLib_Coh_Params mapOp mapSt.
+  Proof.
+    refine {|
+      StLib_StSerialization := map_ser;
+      StLib_Op_Coh := map_op_coh;
+      StLib_St_Coh := map_st_coh; |}.
+    - intros [ol or][ol' or'] v
+        (s & lop & vs & vop & Hseq & Hlopeq & Hveq & Hlopcoh & Hvsq)
+        (s'& lop'& vs'& vop'& Hseq'& Hlopeq'& Hveq'& Hlopcoh'& Hvsq').
+      f_equal; first by simplify_eq/=.
+      simplify_eq/=. by apply (p.(StLib_CohParams).(StLib_Op_Coh_Inj)lop lop' vop').
+    - intros st st' v (l&->&Hl&H'l)(l'&->&Hl'&H'l').
+      assert(l=l') as ->; last reflexivity.
+      rewrite Hl in Hl'. by apply inject_inj.
+    - exact map_coh_ser.
+  Defined.
+
+  Global Instance map_params : StLib_Params mapOp mapSt :=
+    {|
+      StLib_CohParams := map_coh_params;
+      StLib_Denot := map_denot;
+      StLib_Model := map_model;
+    |}.
+
+End Bloup.
+
+Arguments map_params {_ _ _ _ _ _ _ _ _ _}.
 
 Section MapComp_Proof.
   Context (LogOp : Type) (LogSt : Type).
   Context `{!EqDecision LogOp} `{!Countable LogOp}.
-  Context `{!anerisG M Σ}.
-  Context `{!CRDT_Params}.
-  Context `{!Lattice LogSt}.
-  Context `{!Inject LogOp val}.
   Context `{!Inject LogSt val}.
+  Context `{lat : Lattice LogSt}.
+  Context `{a: anerisG M Σ}.
+  Context `{!CRDT_Params}.
   Context `{PA : !StLib_Params LogOp LogSt}.
 
-
-  Global Instance map_params : StLib_Params (mapOp LogOp) (mapSt LogSt).
-  Proof. exact (map_crdt_params LogOp LogSt). Defined.
-
-
   Lemma map_init_st_fn_spec :
-    ⊢ @init_st_fn_spec (mapOp LogOp) (mapSt LogSt) _ _ _ _ _ _ _ map_params
-      map_comb_init_st.
+    ⊢ @init_st_fn_spec (mapOp LogOp) (mapSt LogSt)_ _ _ _ _ _ _ _ map_comb_init_st.
   Proof.
     iIntros (addr).
     iIntros "!#" (Φ) "_ HΦ".
@@ -454,8 +598,8 @@ Section MapComp_Proof.
     iIntros (v Hv).
     iApply "HΦ".
     iPureIntro.
-    by rewrite/StLib_St_Coh/StLib_CohParams/map_params/map_crdt_params
-       /map_crdt_coh_params/map_st_coh/st_crdtM_init_st/StLib_Model/map_crdt_model.
+    by rewrite/StLib_St_Coh/StLib_CohParams/map_params/map_coh_params
+      /map_st_coh/st_crdtM_init_st/StLib_Model/map_model.
   Qed.
 
   Lemma map_mutator_st_spec mut_fn init_fn :
@@ -465,28 +609,6 @@ Section MapComp_Proof.
     @mutator_spec  (mapOp LogOp) (mapSt LogSt) _ _ _ _ _ _ _ map_params
       (λ: "i" "gs" "op", map_comb_mutator init_fn mut_fn "i" "gs" "op").
   Proof.
-    iIntros "#Hinit #Hmut" (addr id st_v op_v s ev op_log st_log)
-                 "!> %φ ((%s'&%lop&%vs&%vop&%Hop1&%Hop2&->&%Hop_coh&->) & (%l_st&->&%Hst_v&%Hst_v') & %Hden & %Hnin & %Hop & %Horig &
-                 %Hmax & %Hevent_ext & %Hcomp) Hφ".
-    do 5 wp_pure _. wp_lam. do 14 wp_pure _.
-    wp_bind (map_lookup _ _)%E.
-    replace (#s') with ($ s'); last done. rewrite Hst_v.
-    iApply (wp_map_lookup with "[]"); first (iPureIntro; by exists l_st).
-    iNext. iIntros (v_st_s').
-    destruct (list_to_map l_st !! s') eqn:E.
-    - iIntros (->).
-      wp_match.
-      wp_apply ("Hmut" with "[]").
-      { iPureIntro. admit. }
-      iIntros (st' (log_st'&Hst'_coh & Hmut)).
-      wp_let.
-      admit.
-    - iIntros (->). do 3 wp_pure _.
-      wp_apply "Hinit"; first trivial. iIntros (vinit Hinit).
-      wp_apply ("Hmut" with "[]").
-      { iPureIntro. admit. }
-      iIntros (st' (log_st'&Hst'_coh & Hmut)).
-      do 2 wp_pure _.
   Admitted.
 
   Lemma map_merge_st_spec merge_fn :
@@ -494,22 +616,6 @@ Section MapComp_Proof.
     @merge_spec _ _ _ _ _ _ _ _ _ map_params
     (λ: "st1" "st2", map_comb_merge merge_fn "st1" "st2").
   Proof.
-    iIntros "#Hmerge" (??????? φ)
-      "!>(%Hst_coh&%Hst_coh'&%Hden&%Hden'&%Hext&%Hcomp&%Hext'&%Hcomp') Hφ".
-    wp_lam. wp_let. wp_lam. wp_pures.
-    wp_apply wp_map_dom; first (iPureIntro; apply Hst_coh).
-    iIntros (v_st_dom Hv_st_dom). wp_let.
-    wp_apply wp_map_dom; first (iPureIntro; apply Hst_coh').
-    iIntros (v_st'_dom Hv_st'_dom). wp_let.
-    wp_apply (wp_set_union); first done.
-    iIntros (v_dom Hv_dom). wp_let.
-    do 3 wp_pure _.
-    wp_bind (map_code.map_empty _)%E.
-    wp_apply wp_map_empty; first trivial. iIntros (st_empty His_empty).
-    wp_smart_apply wp_set_foldl.
-    - admit.
-    - admit.
-    - admit.
   Admitted.
 
   Lemma map_crdt_fun_spec cA :
@@ -538,14 +644,16 @@ Section MapComp_Proof.
         (string_map_ser
             (PA.(StLib_CohParams).(StLib_StSerialization).(s_serializer)).(s_ser))
         (string_map_deser
-            (PA.(StLib_CohParams).(StLib_StSerialization).(s_serializer)).(s_deser)))  -∗
-    @init_spec_for_specific_crdt _ _ _ _ _ _ _ _ map_params.(StLib_Denot) map_params.(StLib_CohParams) _
+            (PA.(StLib_CohParams).(StLib_StSerialization).(s_serializer)).(s_deser))) -∗
+    @init_spec_for_specific_crdt _ _ _ _ _ _ _ _
+      map_params.(StLib_Denot) map_params.(StLib_CohParams) _
       (λ: "addrs" "rid",
          map_comb_init
           (PA.(StLib_CohParams).(StLib_StSerialization).(s_serializer)).(s_ser)
           (PA.(StLib_CohParams).(StLib_StSerialization).(s_serializer)).(s_deser)
-          cA "addrs" "rid")%V.
+          cA "addrs" "rid").
   Proof.
   Admitted.
 
 End MapComp_Proof.
+
